ulib/experimental/FStar.Reflection.Typing.fst
@@ -140,6 +140,7 @@ let rec open_close_inverse' (i:nat) (t:term { ln' t (i - 1) }) (x:var)
     | Tv_FVar _
     | Tv_Type _
     | Tv_Const _
+    | Tv_Unsupp
     | Tv_Unknown
     | Tv_Var _ 
     | Tv_BVar _ -> ()
@@ -369,6 +370,7 @@ let rec close_open_inverse' (i:nat)
     | Tv_FVar _
     | Tv_Type _
     | Tv_Const _
+    | Tv_Unsupp
     | Tv_Unknown
     | Tv_Var _
     | Tv_BVar _ -> ()
@@ -631,6 +633,7 @@ let rec close_with_not_free_var (t:R.term) (x:var) (i:nat)
      | Some tac -> close_with_not_free_var tac x i)
 
   | Tv_Unknown -> ()
+  | Tv_Unsupp -> ()
 
 and close_match_returns_with_not_free_var
   (r:match_returns_ascription)
@@ -786,6 +789,7 @@ let rec open_with_gt_ln e i t j
   | Tv_FVar _
   | Tv_Type _
   | Tv_Const _
+  | Tv_Unsupp
   | Tv_Unknown
   | Tv_Var _
   | Tv_BVar _ -> ()
